floyd/base.v
@@ -3,16 +3,27 @@ Require Export VST.veric.SeparationLogic.
 Require Export VST.msl.Extensionality.
 Require Export compcert.lib.Coqlib.
 Require Export VST.msl.Coqlib2 VST.veric.coqlib4 VST.floyd.coqlib3.
+Require Export VST.veric.juicy_extspec.
+Require Import VST.veric.NullExtension.
 Require Export VST.floyd.jmeq_lemmas.
 Require Export VST.floyd.find_nth_tactic.
-Require Export VST.veric.juicy_extspec.
-(*
-Require VST.veric.SeparationLogicSoundness.
-Export SeparationLogicSoundness.SoundSeparationLogic.MCSL.
-*)
-Require Import VST.veric.NullExtension.
+Require Export VST.floyd.val_lemmas.
+Require Export VST.floyd.assert_lemmas.
+Require VST.floyd.SeparationLogicAsLogicSoundness.
+Export SeparationLogicAsLogicSoundness.MainTheorem.
+Export SeparationLogicAsLogicSoundness.MainTheorem.CSHL_PracticalLogic.
+Export SeparationLogicAsLogicSoundness.MainTheorem.CSHL_PracticalLogic.CSHL_MinimumLogic.
+Export SeparationLogicAsLogicSoundness.MainTheorem.CSHL_PracticalLogic.CSHL_MinimumLogic.CSHL_Def.
+Export SeparationLogicAsLogicSoundness.MainTheorem.CSHL_PracticalLogic.CSHL_MinimumLogic.CSHL_Defs.
 
 Local Open Scope logic.
+
+Definition extract_exists_pre:
+  forall {CS: compspecs} {Espec: OracleKind},
+  forall (A : Type) (P : A -> environ->mpred) c (Delta: tycontext) (R: ret_assert),
+  (forall x, @semax CS Espec Delta (P x) c R) ->
+   @semax CS Espec Delta (EX x:A, P x) c R
+  := @semax_extract_exists.
 
 Arguments alignof_two_p {env} t.
 
@@ -170,82 +181,3 @@ Inductive LLRR : Type :=
   | LLLL : LLRR
   | RRRR : LLRR.
 
-Ltac _destruct_var_types i Heq_vt Heq_ve t b ::=
-  let HH := fresh "H" in
-  match goal with
-  | H: typecheck_var_environ _ _ |- _ =>
-      pose proof WARNING___________you_should_use_tactic___destruct_var_types___instead _ _ H i as HH
-  | H: typecheck_environ _ _ |- _ =>
-      pose proof WARNING___________you_should_use_tactic___destruct_var_types___instead _ _ (proj1 (proj2 H)) i as HH
-  | H: tc_environ _ _ |- _ =>
-      pose proof WARNING___________you_should_use_tactic___destruct_var_types___instead _ _ (proj1 (proj2 H)) i as HH
-  end;
-  match type of HH with
-  | match ?o with _ => _ end =>
-      match goal with
-      | H: o = Some _ |- _ =>
-          rewrite H in HH
-      | H: Some _ = o |- _ =>
-          rewrite <- H in HH
-      | H: o = None |- _ =>
-          rewrite H in HH
-      | H: None = o |- _ =>
-          rewrite <- H in HH
-      | _ =>
-          let HH' := fresh "H" in
-          pose proof eq_refl o as HH';
-          destruct o as [t |] in HH, HH' at 2;
-          pose proof HH' as Heq_vt; clear HH'
-      end
-  end;
-  match type of HH with
-  | ex _ =>
-      pose proof HH as [b Heq_ve]
-  | _ =>
-      pose proof HH as Heq_ve
-  end;
-  clear HH.
-
-Ltac _destruct_glob_types i Heq_gt Heq_ge t b ::=
-  let HH := fresh "H" in
-  match goal with
-  | H: typecheck_glob_environ _ _ |- _ =>
-      pose proof WARNING___________you_should_use_tactic___destruct_glob_types___instead _ _ H i as HH
-  | H: typecheck_environ _ _ |- _ =>
-      pose proof WARNING___________you_should_use_tactic___destruct_glob_types___instead _ _ (proj2 (proj2 H)) i as HH
-  | H: tc_environ _ _ |- _ =>
-      pose proof WARNING___________you_should_use_tactic___destruct_glob_types___instead _ _ (proj2 (proj2 H)) i as HH
-  end;
-  match type of HH with
-  | match ?o with _ => _ end =>
-      match goal with
-      | H: o = Some _ |- _ =>
-          rewrite H in HH
-      | H: Some _ = o |- _ =>
-          rewrite <- H in HH
-      | H: o = None |- _ =>
-          rewrite H in HH
-      | H: None = o |- _ =>
-          rewrite <- H in HH
-      | _ =>
-          let HH' := fresh "H" in
-          pose proof eq_refl o as HH';
-          destruct o as [t |] in HH, HH' at 2;
-          pose proof HH' as Heq_gt; clear HH'
-      end
-  end;
-  match type of HH with
-  | ex _ =>
-      pose proof HH as [b Heq_ge]
-  | _ =>
-      idtac
-  end;
-  clear HH.
-
-(*
-Definition extract_exists_pre:
-  forall {CS: compspecs} {Espec: OracleKind},
-  forall (A : Type) (P : A -> environ->mpred) c (Delta: tycontext) (R: ret_assert),
-  (forall x, @semax CS Espec Delta (P x) c R) ->
-   @semax CS Espec Delta (EX x:A, P x) c R
- := @semax_extract_exists. *)
