floyd/base2.v
@@ -1,9 +1,7 @@
 Require Export VST.floyd.base.
 Require Export VST.floyd.typecheck_lemmas.
 Require Export VST.floyd.functional_base.
-Require Export VST.floyd.val_lemmas.
 Require Export VST.floyd.seplog_tactics.
-Require Export VST.floyd.assert_lemmas.
 Require Export VST.floyd.const_only_eval.
 
 Fixpoint delete_id {A: Type} i (al: list (ident*A)) : option (A * list (ident*A)) :=
